WtLeanIntro/NameGen.lean
@@ -7,21 +7,56 @@ abbrev InScopeVars := Std.HashSet Name
 
 open Std
 
--- theorem term_fresh {n:Nat}: (n != 0) → (sizeOf n - 1 < sizeOf n) := by
---   intro h_succ
---   induction n with
---     | zero => simp[]
---               grind
---     | succ n h_n =>
---         simp
+-- First some helpers for common things
+
+/-- Attaching _x to a name makes it longer -/
+@[simp,grind.]
+theorem name_grows {nm:Name} : nm.length < (nm ++ "_x").length := by
+  have h3: "_x".length = 2 := by rfl
+  simp[*]
+
+/-- Attaching "_x" to a name doesn't preserve equality -/
+@[simp]
+theorem name_append_neq : (x = y ++ "_x") → ¬ x = y := by
+  intro append
+  have _ : x = y → x.toList = y.toList := by exact fun a => congrArg String.toList a
+  cases Classical.em (¬ x = y) with
+    | inl neq => exact neq
+    | inr eq =>
+        have h_1 : y ++ "_x" = x := by grind
+        have h_2 : (y ++ "_x").length = y.length + "_x".length := by simp[String.length_append]
+        have h_3 : y.length < (y ++ "_x").length := by exact name_grows
+        have h_4 : y.length ≠ (y ++ "_x").length := by exact Nat.ne_of_lt h_3
+        have h_5 : y.length = (y ++ "_x").length := by simp_all
+        solve_by_elim
+
+/-- Attaching "_x" to a name doesn't preserve equality -/
+@[simp]
+theorem name_append_neq2 : (x = y ++ "_x") → ¬ x = y := by
+  intro append
+  have _ : x = y → x.toList = y.toList := by exact fun a => congrArg String.toList a
+  if h: ¬ (x = y)
+    then exact h
+    else
+        have h_1 : y ++ "_x" = x := by grind
+        have h_2 : (y ++ "_x").length = y.length + "_x".length := by simp[String.length_append]
+        have h_3 : y.length < (y ++ "_x").length := by exact name_grows
+        have h_4 : y.length ≠ (y ++ "_x").length := by exact Nat.ne_of_lt h_3
+        have h_5 : y.length = (y ++ "_x").length := by simp_all
+        solve_by_elim
+
+/-- Empty set as shown by size=0 has no members -/
+@[simp,grind.]
+theorem emptySet_not_mem {x} {s : InScopeVars}: s.size = 0 → x ∉ s := by
+    intro sz_zero
+    have h1 : s.size == 0 := by exact beq_iff_eq.mpr (by exact sz_zero)
+    have h3 : x ∉ s := by exact HashSet.not_mem_of_isEmpty h1
+    simp[h3]
 
 def findName (n:Nat) (fvs: InScopeVars) (try_name:Name) (h_sz: n = fvs.size): (Name) :=
       if n_zero: n = 0 then
         have _h1 : fvs.size == 0 := by rw[← h_sz]; simp[n_zero]
-        -- have _h2 : fvs.isEmpty = (fvs.size == 0) := by
-        --   exact Std.HashMap.isEmpty_eq_size_eq_zero
         have _empty_helper : fvs.isEmpty := by exact _h1
-
         try_name
       else
         if is_elem: try_name ∈ fvs
@@ -31,77 +66,132 @@ def findName (n:Nat) (fvs: InScopeVars) (try_name:Name) (h_sz: n = fvs.size): (N
                             simp[Std.HashSet.size_erase,is_elem]
             let fvs2 := fvs.erase try_name
             let next_try_name := try_name.append "_x"
+
             findName (n-1) fvs2 next_try_name sz2
           else try_name
   termination_by n
 
-theorem findName_fresh: (findName n fvs try_name h_sz = f_name) → ((f_name = try_name) → (f_name ∉ fvs)) := by
-  intro fn
-  intro name_eq
+/- findName takes in a name suggestion, and variables in scope.
+   It returns a name not yet in scope.
+-/
+def findFreshName (fvs:InScopeVars) (try_name:Name) : Name :=
+  findName (fvs.size) fvs try_name (by rfl)
+
+/-- If the suggested name is not in scope it will be used. -/
+theorem findName_not_elem_eq_try : try_name ∉ fvs → (findName n fvs try_name h_sz = try_name) := by
   fun_induction findName with
-    | case1 h_sz_zero _ empty_hlp =>
-        -- have h1: fvs.isEmpty := by exact empty_hlp
-        (expose_names; exact HashSet.not_mem_of_isEmpty _h1)
-    | case2 fvs try_name h_try_elem ind_fvs ind_fresh_name fvs_non_empty
-        sz_erased
-        i_h =>
-            have h1: f_name ∉ fvs.erase try_name := by grind
+    | case1 _ _a _ =>
+        simp_all
+    | case3 => simp_all
+    | case2 fvs try_name elem_fvs fvs2 next_try_name sz_not_zero
+            sz2 i_hyp  =>
+        have h1: next_try_name = try_name ++ "_x" := by rfl
+        have h2: ¬ next_try_name = try_name := by exact name_append_neq h1
+        simp_all
 
-        -- rw[name_eq]
-        -- simp[h_try_elem]
+/-- Either the suggestion wasn't in scope and we just use it,
+    Or we pick a new name that is:
+      * Not what the user suggested.
+      * Longer than the suggestion.
+      * "Fresh" (Not in scope already)
+      * Since the original suggestion was in scope
+     -/
+@[simp,grind.]
+theorem findName_given_or_longer:
+      (findName n fvs try_name h_sz = f_name) →
+      (try_name ∉ fvs ∨
+          (f_name ≠ try_name ∧
+           f_name.length > try_name.length ∧
+           f_name ∉ fvs ∧
+           try_name ∈ fvs)) := by
+  intro f_name_result
+  cases Classical.em (try_name ∉ fvs) with
+    | inl try_not_elem_fvs =>
+      -- argument used, was not in scope
+      fun_induction findName <;> simp[try_not_elem_fvs]
 
-    | case3 fvs try_name try_n_in _es => rw[name_eq]; simp[try_n_in]
+    | inr nn_try_name_elem_fvs =>
+      have try_name_elem_fvs : try_name ∈ fvs := by simp_all
 
-def freshName (all_fvs: InScopeVars) : (Name × InScopeVars) :=
-    let name := findName (all_fvs.size) all_fvs "x" (by exact rfl)
-    (name,all_fvs.insert name)
+      fun_induction findName with
+        |case1 fvs try_name _ sz_0 h_empty =>
+            have h_not_contains : fvs.contains try_name = false := by refine HashSet.contains_of_isEmpty h_empty
+            have h_not_elem_fvs : try_name ∉ fvs := by simp_all
 
-theorem hs_size_erase_mem {try_name : Name} {fresh_name:Name} {m:InScopeVars}
-    : ((m.erase try_name).size = m.size - 1)
-    → (try_name ∈ m)
-    → (fresh_name ∉ m.erase try_name)
-    → (fresh_name ∉ m)
-    := by intro h_sz
-          intro h_k_mem
-          intro h_x_n_mem
-          have h1: (m.erase try_name).insert try_name = m := by sorry
-          have h2: try_name ∉ m.erase try_name := by simp
-          if h_eq: try_name = fresh_name
-            then
-              grind
-            else
-              grind
+            contradiction --fvs are empty / in set
 
-theorem find_fresh {sz try_name} {fvs:InScopeVars} {h_sz: sz = fvs.size} : (findName sz fvs try_name h_sz) ∉ fvs := by
-  fun_induction findName with
-    | case1 fv2 try_name h_sz =>
-        have h1 : fv2.size == 0 := by exact beq_iff_eq.mpr h_sz
-        -- have h2 : fv2.isEmpty := by exact h1
-        have h3 : try_name ∉ fv2 := by exact HashSet.not_mem_of_isEmpty h1
-        exact h3
-    | case2 fv2 try_name h_try_name_elem
-            h_size_not_null
-            h_sz_smaller
-            h_ind
-             =>
-        let fresh_name := findName (HashSet.size fv2 - 1) (HashSet.erase fv2 try_name) (String.append try_name "_x") h_sz_smaller
-        have h1: findName (HashSet.size fv2 - 1) (HashSet.erase fv2 try_name) (String.append try_name "_x") h_sz_smaller = fresh_name := by rfl
-        rw[h1]
-        have simp_h_ind : (fresh_name ∉ (HashSet.erase fv2 try_name)) := by simp[h_ind,h1,fresh_name]
+        |case3 => contradiction -- in fvs/not in fvs
 
-        -- have h2: fresh_name ≠ try_name := by
+        |case2 fvs try_name h_try_name_elem fvs2 next_try_name sz_fv sz2_fv ind_h  =>
+            have _ : try_name ∈ fvs := by simp[*]
+            have _ : fvs2 = (HashSet.erase fvs try_name) := by grind
+            have h2 : (HashSet.erase fvs try_name).size = fvs2.size := rfl
+            have h_pc : findName (HashSet.size fvs - 1 ) fvs2 next_try_name sz2_fv = f_name := by grind
+            have h_ind_facts: ¬next_try_name      ∈ fvs2 ∨
+                                                      f_name ≠ next_try_name ∧
+                                                      f_name.length > next_try_name.length ∧
+                                                      f_name ∉ fvs2 := by grind
 
+            cases Classical.em (¬next_try_name ∈ fvs2) with
+              |inl next_not_elem =>
+                  have h_1 : ¬next_try_name      ∈ fvs2 := by exact next_not_elem
+                  have h_2: next_try_name = try_name ++ "_x" := by rfl
+                  have h_3: ¬ next_try_name = try_name := by exact name_append_neq h_2
+                  have h_5 : next_try_name      ∉  fvs2 := by exact next_not_elem
 
+                  simp_all
 
-    | case3 => sorry
+                  have h3 : f_name = next_try_name := by
+                    rw[← h_pc]
+                    exact findName_not_elem_eq_try (by grind)
+                  have h8 : next_try_name = String.append try_name "_x" := by rfl
+                  have h8 : next_try_name = try_name ++ "_x" := by rfl
+                  have h9 : next_try_name ≠ try_name := by exact name_append_neq h8
+                  have h9 : f_name ≠ try_name := by simp_all
+                  have h10 : ¬ f_name = try_name := by simp_all
+                  simp[h10]
 
--- theorem fresh_fresh {scope:InScopeVars} : ((freshName scope).fst) ∉ scope := by
---   fun_induction findName with
+                  -- String.length try_name < String.length f_name := by sorry
+                  have h11 : try_name.length < (try_name ++ "_x").length := by exact name_grows
+                  have h12: f_name = (try_name ++ "_x") := by simp[*]
+                  have h13 : try_name.length < f_name.length := by rw [h12]; exact name_grows
+                  simp[h13]
+                  grind
 
-theorem fresh_contains_new {scope:InScopeVars} :
-      (freshName scope) = expanded → ((expanded.fst ∈ expanded.snd) ) := by
-  sorry
+              |inr next_not_elem =>
+                  -- the recursive case!
+                  have h1 : f_name ≠ next_try_name ∧ String.length f_name > next_try_name.length := by grind
+                  have h2 : next_try_name = try_name ++ "_x" := by rfl
+                  have h3 : f_name.length > next_try_name.length := by simp_all
+                  have h4 : try_name.length < (try_name ++ "_x").length := by exact name_grows
+                  have h5 : try_name.length < next_try_name.length := by exact name_grows
+                  have h6 : next_try_name.length < f_name.length := by exact h3
+                  have h7 : try_name.length < f_name.length := by exact Nat.lt_trans h4 h3
+                  have h8 : try_name ≠ f_name := by grind
+                  have h9 : f_name ≠ try_name := by grind
+                  have h10 : ¬ f_name = try_name := by grind
 
-theorem fresh_not_contains_old {scope:InScopeVars} :
-      (freshName scope) = expanded → ((expanded.fst ∉ scope) ) := by
-  sorry
+                  simp [h_try_name_elem, h10,h7]
+                  have h11 : ¬ f_name ∈ fvs := by grind
+
+                  simp[h11]
+
+-- theorem findName_fresh: (findName n fvs try_name h_sz = f_name) → (f_name ∉ fvs) := by
+theorem findName_fresh: (findName n fvs try_name h_sz = f_name) → (f_name ∉ fvs) := by
+  intro name_result
+  have _ : (try_name ∉ fvs ∨
+            (f_name ≠ try_name ∧
+            f_name.length > try_name.length ∧
+            f_name ∉ fvs ∧
+            try_name ∈ fvs)) := by exact findName_given_or_longer name_result
+  cases Classical.em (try_name ∉ fvs) with
+    |inl n_elem =>
+      have h2: (findName n fvs try_name h_sz = try_name) := by exact findName_not_elem_eq_try n_elem
+      have h3 : f_name = try_name := by grind
+      simp_all
+    |inr =>
+      have h2: (f_name ≠ try_name ∧
+            f_name.length > try_name.length ∧
+            f_name ∉ fvs ∧
+            try_name ∈ fvs) := by grind
+      simp[h2]
