WtLeanIntro/Tmp.lean
@@ -2,8 +2,118 @@ import Lean
 
 namespace WtLeanIntro
 
-def xs := ["1"]
+#check Lean.Syntax
 
-def ss := "1"
+open Lean
 
-#eval 1
+def foo : Nat -> Nat
+  | 1 => (1 : Nat)
+  | _ => 2
+
+def isAdd11 : Syntax → Bool
+  | `(Nat.add 1) => true
+  | _ => false
+
+-- def isAdd11 : Syntax → Bool
+--   | `(Nat.add 1 1) => true
+--   | _ => false
+
+#eval isAdd11 (Syntax.mkApp (mkIdent `Nat.add) #[Syntax.mkNumLit "1", Syntax.mkNumLit "1"]) -- true
+#eval isAdd11 (Syntax.mkApp (mkIdent `Nat.add) #[mkIdent `foo, Syntax.mkNumLit "1"]) -- false
+
+-- #eval isAdd11 (Syntax.mkApp (mkIdent `Nat.add) #[(Syntax.mkNumLit "1")])
+-- #eval showTactic (myGrind (1:Nat))
+
+syntax "rep" tactic : tactic
+
+
+
+
+syntax (name := add_ones_n ) "add_ones" : term
+
+@[macro add_ones_n]
+def sasdasdasd : Lean.Macro
+  | `(add_ones) => `(1+1)
+  | _ => Macro.throwUnsupported
+
+
+-- #eval add_ones
+
+-- syntax (name := by_steps_n ) "by_steps" : tactic
+-- syntax (name := by_steps_n1 ) "by_steps" (term) : tactic
+syntax (name := by_steps_many ) "by_steps" (term:lead)+ : tactic
+
+
+-- @[macro by_steps_n1]
+-- def by_stepsImpl : Lean.Macro
+--   | `(tactic | by_steps $t:term ) => `(tactic| have _ : $t := by grind)
+--   | _ => Macro.throwUnsupported
+
+@[macro by_steps_many]
+def by_stepsImplMany : Lean.Macro
+  | `(tactic | by_steps $t:term $ts:term) => do
+      -- let h1 : TSyntax `term := t
+      -- let hs : List (TSyntax `term) := t :: ts.toList
+      let mkHave (hyp:TSyntax `term) : MacroM (TSyntax `tactic)
+            :=`(tactic| have _ : $hyp := by grind; have __a : false = true := by sorry; grind )
+
+      let s1 <- mkHave t
+      let seq <- `(tactic| simp; simp_all; grind)
+      -- let s2 <- `(2)
+      let syn := Syntax.mkSep #[s1,s1] (mkAtom " ")
+      dbg_trace s!"{seq}"
+      return s1
+
+      -- let r := `(tactic| have _ : $t := by grind)
+      -- r
+
+  | _ => Macro.throwUnsupported
+
+#check by_stepsImplMany (Syntax.mkApp (mkIdent `by_steps) #[TSyntax.mk $ mkAtom "true"])
+
+set_option pp.rawOnError true
+
+#check Term
+
+def foob := Syntax
+
+theorem foo2 : 1 + 1 = 2 := by
+  -- simp[]
+  -- have _ : true = true := by grind
+    by_steps (true = true) (true = true)
+
+    -- grind
+
+
+-- (Tactic.tacticHave__
+--  "have"
+--  (Term.letConfig [])
+--  (Term.letDecl
+--   (Term.letIdDecl
+--    (Term.letId (Term.hole "_"))
+--    []
+--    [(Term.typeSpec
+--      ":"
+--      (Term.paren (Term.hygienicLParen "(" (hygieneInfo `[anonymous])) («term_=_» `true "=" `true) ")"))]
+--    ":="
+--    (Term.byTactic
+--     "by"
+--     (Tactic.tacticSeq
+--      (Tactic.tacticSeq1Indented
+--       [(Tactic.grind "grind" (Tactic.optConfig []) [] [] [])
+--        ";"
+--        (Tactic.tacticHave__
+--         "have"
+--         (Term.letConfig [])
+--         (Term.letDecl
+--          (Term.letIdDecl
+--           (Term.letId `__a._@.WtLeanIntro.Tmp.1115644075._hygCtx._hyg.12)
+--           []
+--           [(Term.typeSpec
+--             ":"
+--             («term_=_»
+--              `false._@.WtLeanIntro.Tmp.1115644075._hygCtx._hyg.12
+--              "="
+--              `true._@.WtLeanIntro.Tmp.1115644075._hygCtx._hyg.12))]
+--           ":="
+--           (Term.byTactic "by" (Tactic.tacticSeq (Tactic.tacticSeq1Indented [(Tactic.tacticSorry "sorry")]))))))]))))))
